Good progress on Tailcall

backend/Tailcallproof.v
@@ -222,28 +222,11 @@ Definition regs_inject (j: meminj) (rs1 rs2: Regmap.t val) :=
   forall r,
     Val.inject j (rs1 # r) (rs2 # r).
 
-Lemma meminj_preserves_globals_flat {F V} (g: Genv.t F V) m:
-  Ple (Genv.genv_next g) (Mem.nextblock m) ->
-  meminj_preserves_globals g (Mem.flat_inj (Mem.nextblock m)).
-Proof.
-  intros PLE.
-  split; [|split].
-  - intros id b FS.
-    unfold Genv.find_symbol in FS.
-    eapply Genv.genv_symb_range in FS.
-    unfold Mem.flat_inj; rewrite pred_dec_true; auto. xomega.
-  - intros id b FVI.
-    unfold Genv.find_var_info in FVI.
-    repeat destr_in FVI.
-    eapply Genv.genv_defs_range in Heqo.
-    unfold Mem.flat_inj; rewrite pred_dec_true; auto. xomega.
-  - intros b1 b2 delta gv FVI FI.
-    unfold Genv.find_var_info in FVI.
-    repeat destr_in FVI.
-    eapply Genv.genv_defs_range in Heqo.
-    unfold Mem.flat_inj in FI; destr_in FI. 
-Qed.
-
+Definition inject_globals  {F V} (g: Genv.t F V) j:=
+  (forall b,
+      Plt b (Genv.genv_next g) -> j b = Some (b,0)) /\
+  (forall b1 b2 delta,
+      j b1 = Some (b2, delta) -> Plt b2 (Genv.genv_next g) -> b2 = b1 /\ delta = 0).
 
 Let ge := Genv.globalenv prog.
 Let tge := Genv.globalenv tprog.
@@ -289,18 +272,25 @@ Proof.
 Qed.
 
 Lemma find_function_translated:
-  forall ros rs rs' f m,
+  forall ros rs rs' f j,
   find_function ge ros rs = Some f ->
-  regs_inject (Mem.flat_inj (Mem.nextblock m)) rs rs' ->
+  regs_inject j rs rs' ->
+  inject_globals ge j ->
   find_function tge ros rs' = Some (transf_fundef f).
 Proof.
-  intros until m; destruct ros; simpl.
-  intros.
+  intros ros rs rs' f j FF RI IG; destruct ros; simpl in *.
   assert (rs'#r = rs#r).
+  {
     exploit Genv.find_funct_inv; eauto. intros [b EQ].
-    generalize (H0 r). rewrite EQ. intro LD. inv LD.
-    unfold Mem.flat_inj in H4. repeat destr_in H4. reflexivity.
-  rewrite H1. apply functions_translated; auto.
+    generalize (RI r). rewrite EQ. intro LD. inv LD.
+    rewrite EQ in FF.
+    unfold Genv.find_funct in FF; repeat destr_in FF.
+    unfold Genv.find_funct_ptr in H0. repeat destr_in H0.
+    eapply Genv.genv_defs_range in Heqo.
+    destruct IG as (IG1 & IG2).
+    erewrite IG1 in H2; eauto. inv H2. reflexivity.
+  } 
+  rewrite H. apply functions_translated; auto.
   rewrite symbols_preserved. destruct (Genv.find_symbol ge i); intros.
   apply funct_ptr_translated; auto.
   discriminate.
@@ -347,13 +337,13 @@ to specify the shape of the stack injection function [g]. *)
 Inductive match_stackframes: meminj -> list bool -> list stackframe -> list stackframe -> Prop :=
   | match_stackframes_nil j:
       match_stackframes j nil nil nil
-  | match_stackframes_normal: forall j l stk stk' res sp pc rs rs' f,
+  | match_stackframes_normal: forall j l stk stk' res sp sp' pc rs rs' f,
       match_stackframes j l stk stk' ->
       regs_inject j rs rs' ->
-      j sp = Some (sp,0) ->
+      j sp = Some (sp',0) ->
       match_stackframes j (true::l)
         (Stackframe res f (Vptr sp Ptrofs.zero) pc rs :: stk)
-        (Stackframe res (transf_function f) (Vptr sp Ptrofs.zero) pc rs' :: stk')
+        (Stackframe res (transf_function f) (Vptr sp' Ptrofs.zero) pc rs' :: stk')
   | match_stackframes_tail: forall j l stk stk' res sp pc rs f,
       match_stackframes j l stk stk' ->
       is_return_spec f pc res ->
@@ -397,37 +387,43 @@ Qed.
 
 Inductive match_states: state -> state -> Prop :=
   | match_states_normal:
-      forall s sp pc rs m s' rs' m' f g l
-             (STACKS: match_stackframes (Mem.flat_inj (Mem.nextblock m)) l s s')
-             (RLD: regs_inject (Mem.flat_inj (Mem.nextblock m)) rs rs')
-             (MLD: Mem.inject (Mem.flat_inj (Mem.nextblock m)) g m m')
-             (CFG: compat_frameinj (true::l) g),
+      forall s sp sp' pc rs m s' rs' m' f g l j
+
+             (STACKS: match_stackframes j l s s')
+             (RLD: regs_inject j rs rs')
+             (MLD: Mem.inject j g m m')
+             (CFG: compat_frameinj (true::l) g)
+             (IG: inject_globals ge j)
+             (JB: j sp = Some (sp', 0)),
       match_states (State s f (Vptr sp Ptrofs.zero) pc rs m)
-                   (State s' (transf_function f) (Vptr sp Ptrofs.zero) pc rs' m')
+                   (State s' (transf_function f) (Vptr sp' Ptrofs.zero) pc rs' m')
   | match_states_call:
-      forall s f args m s' args' m' sz g l
-        (MS: match_stackframes (Mem.flat_inj (Mem.nextblock m)) l s s')
-        (LDargs: Val.inject_list (Mem.flat_inj (Mem.nextblock m)) args args')
-        (MLD: Mem.inject (Mem.flat_inj (Mem.nextblock m)) g m m')
-        (CFG: compat_frameinj l g),
+      forall s f args m s' args' m' sz g l j
+        (MS: match_stackframes j l s s')
+        (LDargs: Val.inject_list j args args')
+        (MLD: Mem.inject j g m m')
+        (CFG: compat_frameinj l g)
+        (IG: inject_globals ge j),
       match_states (Callstate s f args m sz)
                    (Callstate s' (transf_fundef f) args' m' sz)
   | match_states_return:
-      forall s v m s' v' m' g l
-        (MS: match_stackframes (Mem.flat_inj (Mem.nextblock m)) l s s')
-        (LDret: Val.inject (Mem.flat_inj (Mem.nextblock m)) v v')
-        (MLD: Mem.inject (Mem.flat_inj (Mem.nextblock m)) g m m')
-        (CFG: compat_frameinj (true::l) g),
+      forall s v m s' v' m' g l j
+        (MS: match_stackframes j l s s')
+        (LDret: Val.inject j v v')
+        (MLD: Mem.inject j g m m')
+        (CFG: compat_frameinj l g)
+             (IG: inject_globals ge j),
         match_states (Returnstate s v m)
                      (Returnstate s' v' m')
   | match_states_interm:
-      forall s sp pc rs m s' m' f r v' g l
-             (STACKS: match_stackframes (Mem.flat_inj (Mem.nextblock m)) l s s')
-             (MLD: Mem.inject (Mem.flat_inj (Mem.nextblock m)) g m m')
+      forall s sp pc rs m s' m' f r v' g l j
+             (STACKS: match_stackframes j l s s')
+             (MLD: Mem.inject j g m m')
              (RETspec: is_return_spec f pc r)
              (SZzero: f.(fn_stacksize) = 0)
-             (LDret: Val.inject (Mem.flat_inj (Mem.nextblock m)) (rs#r) v')
-             (CFG: compat_frameinj l g),
+             (LDret: Val.inject j (rs#r) v')
+             (CFG: compat_frameinj (false::l) g)
+             (IG: inject_globals ge j),
         match_states (State s f (Vptr sp Ptrofs.zero) pc rs m)
                      (Returnstate s' v' m').
 
@@ -559,7 +555,7 @@ Variable fn_stack_requirements: ident -> Z.
 
 Lemma ros_is_function_transf:
   forall j ros rs rs' id,
-    meminj_preserves_globals ge j ->
+    inject_globals ge j ->
     ros_is_function ge ros rs id ->
     regs_inject j rs rs' ->
     ros_is_function tge ros rs' id.
@@ -571,12 +567,31 @@ Proof.
   eexists; eexists; split; eauto.
   rewrite symbols_preserved. rewrite FS.
   f_equal.
-  destruct H. apply H in FS. rewrite FS in H4; inv H4. auto.
+  destruct H. erewrite H in H4. inv H4. auto. 
+  eapply Genv.genv_symb_range; eauto.
+Qed.
+
+Lemma inject_globals_meminj_preserves_globals:
+  forall {F V} (g: Genv.t F V) j,
+    inject_globals g j ->
+    meminj_preserves_globals g j.
+Proof.
+  intros F V g j (IG1 & IG2); split; [|split].
+  - intros id b FS.
+    eapply IG1. eapply Genv.genv_symb_range; eauto.
+  - intros b gv FVI.
+    unfold Genv.find_var_info in FVI.
+    repeat destr_in FVI.
+    eapply IG1. eapply Genv.genv_defs_range; eauto.
+  - intros b1 b2 delta gv FVI JB.
+    unfold Genv.find_var_info in FVI.
+    repeat destr_in FVI.
+    eapply IG2 in JB; eauto. apply JB. eapply Genv.genv_defs_range; eauto.
 Qed.
 
 Lemma transf_step_correct:
   forall s1 t s2, step fn_stack_requirements ge s1 t s2 ->
-  forall s1' (MS: match_states s1 s1') (MSG: match_state_ge ge s1) (SPV: sp_valid s1) (MSA: match_stack_adt s1) (MSA': match_stack_adt s1'),
+  forall s1' (MS: match_states s1 s1') (MSG: match_state_ge ge s1) (MSG': match_state_ge tge s1') (SPV: sp_valid s1) (MSA: match_stack_adt s1) (MSA': match_stack_adt s1'),
   (exists s2', step fn_stack_requirements tge s1' t s2' /\ match_states s2 s2')
   \/ (measure s2 < measure s1 /\ t = E0 /\ match_states s2 s1')%nat.
 Proof.
@@ -592,13 +607,11 @@ Proof.
 
 - (* op *)
   TransfInstr.
-  assert (Val.inject_list (Mem.flat_inj (Mem.nextblock m)) (rs##args) (rs'##args)). apply regs_inject_regs; auto.
+  assert (Val.inject_list j (rs##args) (rs'##args)). apply regs_inject_regs; auto.
   exploit eval_operation_inject; eauto.
-  eapply meminj_preserves_globals_flat; eauto.
-  unfold Mem.flat_inj. rewrite pred_dec_true. reflexivity.
-  inv SPV. eauto.
+  eapply inject_globals_meminj_preserves_globals; eauto.
   intros [v' [EVAL' VLD]].
-  left. exists (State s' (transf_function f) (Vptr sp0 Ptrofs.zero) pc' (rs'#res <- v') m'); split.
+  left. exists (State s' (transf_function f) (Vptr sp' Ptrofs.zero) pc' (rs'#res <- v') m'); split.
   eapply exec_Iop; eauto.  rewrite <- EVAL'.
   rewrite eval_shift_stack_operation.
   apply eval_operation_preserved. exact symbols_preserved.
@@ -610,14 +623,13 @@ Proof.
 
 - (* load *)
   TransfInstr.
-  assert (Val.inject_list (Mem.flat_inj (Mem.nextblock m)) (rs##args) (rs'##args)). apply regs_inject_regs; auto.
+  assert (Val.inject_list j (rs##args) (rs'##args)). apply regs_inject_regs; auto.
   exploit eval_addressing_inject; eauto.
-  eapply meminj_preserves_globals_flat; eauto.
-  unfold Mem.flat_inj; rewrite pred_dec_true; auto.   inv SPV. eauto.
+  eapply inject_globals_meminj_preserves_globals; eauto.
   intros [a' [ADDR' ALD]].
   exploit Mem.loadv_inject; eauto.
   intros [v' [LOAD' VLD]].
-  left. exists (State s' (transf_function f) (Vptr sp0 Ptrofs.zero) pc' (rs'#dst <- v') m'); split.
+  left. exists (State s' (transf_function f) (Vptr sp' Ptrofs.zero) pc' (rs'#dst <- v') m'); split.
   eapply exec_Iload with (a0 := a'). eauto.  rewrite <- ADDR'.
   rewrite eval_shift_stack_addressing.
   apply eval_addressing_preserved. exact symbols_preserved. eauto.
@@ -625,28 +637,24 @@ Proof.
 
 - (* store *)
   TransfInstr.
-  assert (Val.inject_list (Mem.flat_inj (Mem.nextblock m)) (rs##args) (rs'##args)). apply regs_inject_regs; auto.
+  assert (Val.inject_list j (rs##args) (rs'##args)). apply regs_inject_regs; auto.
   exploit eval_addressing_inject; eauto.
-  eapply meminj_preserves_globals_flat; eauto.
-  unfold Mem.flat_inj; rewrite pred_dec_true; auto. inv SPV. eauto.
+  eapply inject_globals_meminj_preserves_globals; eauto.
   intros [a' [ADDR' ALD]].
   exploit Mem.storev_mapped_inject. 2: eexact H1. eauto. eauto. apply RLD.
   intros [m'1 [STORE' MLD']].
-  left. exists (State s' (transf_function f) (Vptr sp0 Ptrofs.zero) pc' rs' m'1); split.
+  left. exists (State s' (transf_function f) (Vptr sp' Ptrofs.zero) pc' rs' m'1); split.
   eapply exec_Istore with (a0 := a'). eauto.  rewrite <- ADDR'.
   rewrite eval_shift_stack_addressing.
   apply eval_addressing_preserved. exact symbols_preserved. eauto.
   destruct a; simpl in H1; try discriminate.
   econstructor; eauto.
-  erewrite Mem.nextblock_store; eauto.
-  erewrite Mem.nextblock_store; eauto.
-  erewrite Mem.nextblock_store; eauto.
 
 - (* call *)
   exploit find_function_translated; eauto. intro FIND'.
   TransfInstr.
 + (* call turned tailcall *)
-  assert (X: { m'' | Mem.free m' sp0 0 (fn_stacksize (transf_function f)) = Some m''}).
+  assert (X: { m'' | Mem.free m' sp' 0 (fn_stacksize (transf_function f)) = Some m''}).
   {
     apply Mem.range_perm_free. rewrite stacksize_preserved. rewrite H7.
     red; intros; omegaContradiction.
@@ -678,7 +686,7 @@ Proof.
   trim UINJ.
   {
     red in CFG. simpl in CFG.
-    intros i j Gi LT.
+    intros i1 i2 Gi LT.
     eapply compat_frameinj_rec_above in Gi. 2: apply CFG. omega. omega.
   }
   trim UINJ. apply CFG.
@@ -687,7 +695,6 @@ Proof.
   eapply exec_Itailcall; eauto.
   {
     eapply ros_is_function_transf; eauto.
-    eapply meminj_preserves_globals_flat; eauto.
   }
   apply sig_preserved.
   econstructor. eapply match_stackframes_tail; eauto. apply regs_inject_regs; auto.
@@ -731,27 +738,25 @@ Proof.
 
   }
 
+  eauto.
+
 + (* call that remains a call *)
-  left. exists (Callstate (Stackframe res (transf_function f) (Vptr sp0 Ptrofs.zero) pc' rs' :: s')
+  left. exists (Callstate (Stackframe res (transf_function f) (Vptr sp' Ptrofs.zero) pc' rs' :: s')
                           (transf_fundef fd) (rs'##args) m' (fn_stack_requirements id)); split.
   eapply exec_Icall; eauto.
   eapply ros_is_function_transf; eauto.
-  eapply meminj_preserves_globals_flat; eauto.
   apply sig_preserved.
-  econstructor. constructor; eauto.
-  unfold Mem.flat_inj; rewrite pred_dec_true. auto. inv SPV; auto.
-  apply regs_inject_regs; auto. eauto.
-  auto.
+  econstructor; eauto. constructor; eauto.
+  apply regs_inject_regs; auto. 
 
 - (* tailcall *)
   exploit find_function_translated; eauto. intro FIND'.
-  exploit Mem.free_parallel_inject; eauto.
-  unfold Mem.flat_inj; rewrite pred_dec_true; auto. inv SPV; auto. constructor.
+  exploit Mem.free_parallel_inject; eauto. constructor.
   intros [m'1 [FREE EXT]].
   exploit Mem.unrecord_stack_block_inject_parallel. apply EXT. eauto.
   {
     red in CFG. simpl in CFG.
-    intros i j Gi LT.
+    intros i1 i2 Gi LT.
     eapply compat_frameinj_rec_above in Gi. 2: apply CFG. omega. omega.
   }
   {
@@ -762,17 +767,10 @@ Proof.
   left. exists (Callstate s' (transf_fundef fd) (rs'##args) m2' (fn_stack_requirements id)); split.
   eapply exec_Itailcall; eauto.
   eapply ros_is_function_transf; eauto.
-  eapply meminj_preserves_globals_flat; eauto.
   apply sig_preserved.
-  eauto. rewrite stacksize_preserved; auto. rewrite ! Z.add_0_r in FREE. eauto.
-  econstructor.
-  erewrite Mem.unrecord_stack_block_nextblock by eauto.
-  erewrite Mem.nextblock_free by eauto. eauto.
-  eauto.  apply regs_inject_regs; auto.
-  erewrite Mem.unrecord_stack_block_nextblock by eauto.
-  erewrite Mem.nextblock_free by eauto. eauto.
-  erewrite Mem.unrecord_stack_block_nextblock by eauto.
-  erewrite Mem.nextblock_free by eauto. eauto.
+  rewrite stacksize_preserved; auto. rewrite ! Z.add_0_r in FREE. eauto.
+  econstructor; eauto.
+  apply regs_inject_regs; auto.
   {
     destruct CFG as (G0 & CFG).
 
@@ -792,111 +790,280 @@ Proof.
           * unfold option_map. rewrite Gn. reflexivity.
           * eapply IHl; eauto.
     Qed.
-    eapply compat_frameinj_rec_pop_parallel; eauto.
 
+    eapply compat_frameinj_rec_pop_parallel; eauto.
   }
 
 - (* builtin *)
   TransfInstr.
   exploit (@eval_builtin_args_inject _ _ _ _ ge tge (fun r => rs#r) (fun r => rs'#r) (Vptr sp0 Ptrofs.zero)); eauto.
   {
-    econstructor. unfold Mem.flat_inj. rewrite pred_dec_true; eauto. inv SPV; auto. reflexivity.
-  }
-  {
     simpl. intros; rewrite symbols_preserved; auto.
   }
   {
     simpl; intros.
-    generalize (meminj_preserves_globals_flat ge m). intro MPG. trim MPG; eauto.
-    destruct MPG; eauto.
+    eapply IG; eauto. eapply Genv.genv_symb_range; eauto.
   }
   intros (vargs' & P & Q).
   exploit external_call_mem_inject; eauto.
-  eapply meminj_preserves_globals_flat; eauto.
+  eapply inject_globals_meminj_preserves_globals; eauto.
   intros [f' [v' [m'1 [A [B [C [D [E [F G]]]]]]]]].
-  left. exists (State s' (transf_function f) (Vptr sp0 Ptrofs.zero) pc' (regmap_setres res v' rs') m'1); split.
+  left. exists (State s' (transf_function f) (Vptr sp' Ptrofs.zero) pc' (regmap_setres res v' rs') m'1); split.
   eapply exec_Ibuiltin; eauto.
-  edestruct eval_builtin_args_inject with (e1:= fun r => rs # r) (e2:= fun r => rs' # r) (sp1:=Vptr sp0 Ptrofs.zero) as
-      (args' & EVALargs' & INJargs); eauto.
-  {
-    econstructor. unfold Mem.flat_inj.  rewrite pred_dec_true; eauto. inv SPV; auto. reflexivity.
-  }
-  {
-    simpl; intros.
-    generalize (meminj_preserves_globals_flat ge m). intro MPG. trim MPG; eauto.
-    destruct MPG; eauto.
-  }
   eapply external_call_symbols_preserved; eauto. apply senv_preserved.
-  econstructor; eauto.
-  
+  econstructor. 3: eauto.
+  all: eauto.
+
+  Lemma match_stackframes_incr:
+    forall f l s s'
+      (MS: match_stackframes f l s s')
+      f' (INCR: inject_incr f f'),
+      match_stackframes f' l s s'.
+  Proof.
+    induction 1; simpl; intros; eauto; try now econstructor; eauto.
+    econstructor; eauto.
+    red; intros; eauto.
+  Qed.
+  eapply match_stackframes_incr; eauto.
   apply set_res_inject; auto.
+  red; intros; eauto.
+
+  Lemma inject_globals_incr:
+    forall f f'
+      (INCR : inject_incr f f')
+      (SEP : forall b1 b2 delta, f b1 = None -> f' b1 = Some (b2, delta) -> Ple (Genv.genv_next ge) b1 /\ Ple (Genv.genv_next ge) b2)
+      (IG: inject_globals ge f),
+      inject_globals ge f'.
+  Proof.
+    intros f f' INCR SEP (IG1 & IG2); split; intros; eauto.
+    eapply IG2; eauto.
+    destruct (f b1) eqn:FB1.
+    - destruct p. eapply INCR in FB1. congruence.
+    - specialize (SEP _ _ _ FB1 H).
+      xomega.
+  Qed.
+  eapply inject_globals_incr; eauto.
+  intros.
+  specialize (G _ _ _ H2 H3). unfold Mem.valid_block in G.
+  red in MSG. simpl in MSG.
+  red in MSG'. simpl in MSG'.
+  rewrite genv_next_preserved in MSG'. xomega.
 
 - (* cond *)
   TransfInstr.
-  left. exists (State s' (transf_function f) (Vptr sp0 Ptrofs.zero) (if b then ifso else ifnot) rs' m'); split.
+  left. exists (State s' (transf_function f) (Vptr sp' Ptrofs.zero) (if b then ifso else ifnot) rs' m'); split.
   eapply exec_Icond; eauto.
-  apply eval_condition_inject with (rs##args) m; auto. apply regs_inject_regs; auto.
-  constructor; auto.
+  eapply eval_condition_inject. apply regs_inject_regs; auto.
+  eauto. eauto. auto.
+  econstructor; eauto.
 
 - (* jumptable *)
   TransfInstr.
-  left. exists (State s' (transf_function f) (Vptr sp0 Ptrofs.zero) pc' rs' m'); split.
+  left. exists (State s' (transf_function f) (Vptr sp' Ptrofs.zero) pc' rs' m'); split.
   eapply exec_Ijumptable; eauto.
   generalize (RLD arg). rewrite H0. intro. inv H2. auto.
-  constructor; auto.
+  econstructor; eauto.
 
 - (* return *)
-  exploit Mem.free_parallel_inject; eauto. intros [m'1 [FREE EXT]].
+  exploit Mem.free_parallel_inject; eauto. constructor. intros [m'1 [FREE EXT]].
+  exploit Mem.unrecord_stack_block_inject_parallel. apply EXT. eauto.
+  {
+    red in CFG. simpl in CFG.
+    intros i1 i2 Gi LT.
+    eapply compat_frameinj_rec_above in Gi. 2: apply CFG. omega. omega.
+  }
+  {
+    apply CFG.
+  }
+  intros (m2' & USB' & UINJ).
   TransfInstr.
-  left. exists (Returnstate s' (regmap_optget or Vundef rs') m'1); split.
-  apply exec_Ireturn; auto. rewrite stacksize_preserved; auto.
-  constructor. auto.
+  left. exists (Returnstate s' (regmap_optget or Vundef rs') m2'); split.
+  eapply exec_Ireturn; eauto.
+  rewrite stacksize_preserved; auto. rewrite ! Z.add_0_r in FREE. eauto.
+  econstructor; eauto.
   destruct or; simpl. apply RLD. constructor.
   auto.
+  destruct CFG as (G0 & CFG).
+  eapply compat_frameinj_rec_pop_parallel; eauto.
 
 - (* eliminated return None *)
   assert (or = None) by congruence. subst or.
   right. split. simpl. omega. split. auto.
-  constructor. auto.
-  simpl. constructor.
-  eapply Mem.free_left_inject; eauto.
+  econstructor. eauto. simpl. constructor.
+  eapply Mem.unrecord_stack_block_inject_left'.
+  eapply Mem.free_left_inject; eauto. eauto.
+  apply CFG.
+  erewrite Mem.free_stack_blocks; eauto.
+  destruct MSA as (sprog & sinit & EQstk & LF2).
+  inv LF2. simpl in EQstk.
+  rewrite EQstk. unfold is_stack_top. simpl.
+  destruct H6 as (frameblocks & PERM).
+  rewrite frameblocks. intros b [|[]]; subst.
+  intros o k p P.
+  rewrite Mem.perm_free in P; eauto.
+  destruct P as (P & Q).
+  intuition. apply PERM in Q. intuition.
+
+
+  red; red in CFG.
+  simpl in CFG.
+  destruct CFG as (G0 & CFG).
+
+  Lemma compat_frameinj_rec_pop_left:
+    forall g l ns nt
+      (CF: compat_frameinj_rec l g (S ns) nt),
+      compat_frameinj_rec l (fun n : nat => g (S n)) ns nt.
+  Proof.
+    induction l; simpl; intros; eauto.
+    - eapply CF in Gi; eauto. omega.
+    - destruct a; destruct CF as [Gn CF].
+      + split; auto.
+      + split; auto.
+  Qed.
+
+  eapply compat_frameinj_rec_pop_left; eauto.
+  auto.
 
 - (* eliminated return Some *)
   assert (or = Some r) by congruence. subst or.
   right. split. simpl. omega. split. auto.
-  constructor. auto.
+  econstructor. eauto.
   simpl. auto.
-  eapply Mem.free_left_inject; eauto.
+  eapply Mem.unrecord_stack_block_inject_left'.
+  eapply Mem.free_left_inject; eauto. eauto.
+  apply CFG.
+  erewrite Mem.free_stack_blocks; eauto.
+  destruct MSA as (sprog & sinit & EQstk & LF2).
+  inv LF2. simpl in EQstk.
+  rewrite EQstk. unfold is_stack_top. simpl.
+  destruct H6 as (frameblocks & PERM).
+  rewrite frameblocks. intros b [|[]]; subst.
+  intros o k p P.
+  rewrite Mem.perm_free in P; eauto.
+  destruct P as (P & Q).
+  intuition. apply PERM in Q. intuition.
+  red; red in CFG.
+  simpl in CFG.
+  destruct CFG as (G0 & CFG).
+  eapply compat_frameinj_rec_pop_left; eauto.
+  auto.
 
 - (* internal call *)
-  exploit Mem.alloc_inject; eauto.
-    instantiate (1 := 0). omega.
-    instantiate (1 := fn_stacksize f). omega.
-  intros [m'1 [ALLOC EXT]].
-  assert (fn_stacksize (transf_function f) = fn_stacksize f /\
-          fn_entrypoint (transf_function f) = fn_entrypoint f /\
-          fn_params (transf_function f) = fn_params f).
-    unfold transf_function. destruct (zeq (fn_stacksize f) 0); auto.
-  destruct H0 as [EQ1 [EQ2 EQ3]].
-  left. econstructor; split.
-  simpl. eapply exec_function_internal; eauto. rewrite EQ1; eauto.
-  rewrite EQ2. rewrite EQ3. constructor; auto.
-  apply regs_inject_init_regs. auto.
+  exploit Mem.alloc_parallel_inject; eauto.
+  + instantiate (1 := 0). omega.
+  + instantiate (1 := fn_stacksize f). omega.
+  + intros [f' [m'1 [b2 [ALLOC [INJ [INCR [FEQ FOLD]]]]]]].
+    assert (EQ: fn_stacksize (transf_function f) = fn_stacksize f /\
+                fn_entrypoint (transf_function f) = fn_entrypoint f /\
+                fn_params (transf_function f) = fn_params f).
+    {
+      unfold transf_function. destruct (zeq (fn_stacksize f) 0); auto.
+    }
+    destruct EQ as [EQ1 [EQ2 EQ3]].
+    exploit Mem.record_stack_blocks_inject_parallel. apply INJ. 7: eauto.
+    instantiate (1 := make_singleton_frame_adt b2 (fn_stacksize f) sz).
+    * red. red. simpl. constructor; auto. simpl. rewrite FEQ.
+      intros b0 delta A. inv A. rewrite pred_dec_true; auto.
+      eexists; split; eauto.
+      split; simpl; auto. intros; omega.
+    * unfold in_frame; simpl.
+      erewrite Mem.alloc_stack_blocks; eauto.
+      intros b IFR [|[]]; subst.
+      eapply Mem.in_frames_valid in IFR. eapply Mem.fresh_block_alloc in IFR; eauto.
+    * red.
+      intros b [|[]]; subst. simpl.
+      eapply Mem.valid_new_block; eauto.
+    * intros b fi [A|[]]; inv A. simpl.
+      intros; eapply Mem.perm_alloc_3; eauto.
+    * intros b1 b0 delta FB.
+      unfold in_frame; simpl.
+      split; intros [|[]]; subst; left. congruence.
+      destruct (peq stk b1); auto. rewrite FOLD in FB; auto.
+      eapply Mem.valid_block_inject_2 in FB; eauto.
+      eapply Mem.fresh_block_alloc in FB; eauto. easy.
+    * reflexivity.
+    * intros (m2' & RSB & UINJ).
+      left. econstructor; split.
+      -- simpl. eapply exec_function_internal; eauto. rewrite EQ1; eauto.
+         rewrite EQ1; eauto.
+      -- rewrite EQ2. rewrite EQ3. econstructor. 3: eauto.
+         all: eauto.
+         eapply match_stackframes_incr; eauto.
 
+         Lemma regs_inject_init_regs:
+           forall j params vl vl',
+             Val.inject_list j vl vl' ->
+             regs_inject j (init_regs vl params) (init_regs vl' params).
+         Proof.
+           induction params; intros.
+           simpl. red; intros. rewrite Regmap.gi. constructor.
+           simpl. inv H.   red; intros. rewrite Regmap.gi. constructor.
+           apply set_reg_inject. auto. auto.
+         Qed.
+
+         apply regs_inject_init_regs. auto.
+         eapply val_inject_list_incr; eauto.
+
+
+         red in CFG; red. simpl. split; auto.
+
+         Lemma compat_frameinj_rec_push_parallel:
+           forall g l ns nt
+             (CFR: compat_frameinj_rec l g ns nt)
+             g'
+             (G'spec: forall i, (S ns <= i)%nat -> g' i = option_map S (g (pred i))),
+             compat_frameinj_rec l g' (S ns) (S nt).
+         Proof.
+           induction l; simpl; intros; eauto.
+           - rewrite G'spec in Gi; auto.
+             unfold option_map in Gi; repeat destr_in Gi.
+             eapply CFR in Heqo. omega. omega. 
+           - destr; destruct CFR as (Gn & CFR).
+             + split.
+               * rewrite G'spec; auto.
+                 unfold option_map. simpl. rewrite Gn. reflexivity.
+               * eapply IHl; eauto.
+                 intros; apply G'spec. omega.
+             + split.
+               * rewrite G'spec; auto.
+                 unfold option_map. simpl. rewrite Gn. reflexivity.
+               * eapply IHl; eauto.
+                 intros; apply G'spec. omega.
+         Qed.
+         eapply compat_frameinj_rec_push_parallel; eauto.
+         intros; destr. omega.
+         eapply inject_globals_incr; eauto.
+         intros.
+         destruct (peq b1 stk). subst. rewrite FEQ in H2; inv H2.
+         red in MSG. simpl in MSG.
+         red in MSG'. simpl in MSG'.
+         rewrite genv_next_preserved in MSG'.
+         apply Mem.alloc_result in H. apply Mem.alloc_result in ALLOC. subst. xomega.
+         rewrite FOLD in H2. congruence. auto.
+         
 - (* external call *)
   exploit external_call_mem_inject; eauto.
-  intros [res' [m2' [A [B [C D]]]]].
+  eapply inject_globals_meminj_preserves_globals; eauto.
+  intros [f' [res' [m2' [A [B [C [D [E [F G]]]]]]]]].
   left. exists (Returnstate s' res' m2'); split.
-  simpl. econstructor; eauto.
+  econstructor; eauto.
   eapply external_call_symbols_preserved; eauto. apply senv_preserved.
-  constructor; auto.
+  econstructor. 3: eauto.
+  all: eauto.
+  eapply match_stackframes_incr; eauto.
+  eapply inject_globals_incr; eauto.
+  intros.
+  specialize (G _ _ _ H0 H1). unfold Mem.valid_block in G.
+  red in MSG. simpl in MSG.
+  red in MSG'. simpl in MSG'.
+  rewrite genv_next_preserved in MSG'. xomega.
 
 - (* returnstate *)
-  inv H2.
+  inv MS0.
 + (* synchronous return in both programs *)
   left. econstructor; split.
   apply exec_return.
-  constructor; auto. apply set_reg_inject; auto.
+  econstructor; eauto. apply set_reg_inject; auto.
 + (* return instr in source program, eliminated because of tailcall *)
   right. split. unfold measure. simpl length.
   change (S (length s) * (niter + 2))%nat
